disk-betree/BucketWeights.i.dfy
@@ -1,0 +1,105 @@
+include "BucketsLib.i.dfy"
+
+module BucketWeights {
+  import opened PivotsLib
+  import opened Lexicographic_Byte_Order
+  import opened ValueMessage
+  import ValueWithDefault
+  import opened Maps
+  import opened Sequences
+  import opened BucketsLib
+
+  function WeightKey(key: Key) : int
+  {
+    8 + |key|
+  }
+ 
+  function WeightKeySeq(keys: seq<Key>) : int
+  {
+    if |keys| == 0 then 0 else WeightKeySeq(DropLast(keys)) + WeightKey(Last(keys))
+  }
+
+  function WeightMessage(msg: Message) : int
+  {
+    match msg {
+      case Define(value) => ValueWithDefault.Len(value)
+      case Update(delta) => 0
+    }
+  }
+
+  function WeightMessageSeq(msgs: seq<Message>) : int
+  {
+    if |msgs| == 0 then 0 else WeightMessageSeq(DropLast(msgs)) + WeightMessage(Last(msgs))
+  }
+
+  function {:opaque} ChooseKey(bucket: Bucket) : (key : Key)
+  requires |bucket| > 0
+  ensures key in bucket
+  {
+    var key :| key in bucket;
+    key
+  }
+
+  function {:opaque} WeightBucket(bucket: Bucket) : int
+  {
+    if |bucket| == 0 then 0 else (
+      var key := ChooseKey(bucket);
+      var msg := bucket[key];
+      WeightBucket(MapRemove1(bucket, key)) + WeightKey(key) + WeightMessage(msg)
+    )
+  }
+
+  function {:opaque} WeightBucketList(buckets: BucketList) : int
+  {
+    if |buckets| == 0 then 0 else (
+      WeightBucketList(DropLast(buckets)) + WeightBucket(Last(buckets))
+    )
+  }
+
+  lemma WeightSplitBucketListLeft(blist: BucketList, pivots: seq<Key>, cLeft: int, key: Key)
+  requires SplitBucketListLeft.requires(blist, pivots, cLeft, key)
+  ensures WeightBucketList(SplitBucketListLeft(blist, pivots, cLeft, key))
+      <= WeightBucketList(blist)
+
+  lemma WeightSplitBucketListRight(blist: BucketList, pivots: seq<Key>, cRight: int, key: Key)
+  requires SplitBucketListRight.requires(blist, pivots, cRight, key)
+  ensures WeightBucketList(SplitBucketListRight(blist, pivots, cRight, key))
+      <= WeightBucketList(blist)
+
+  lemma WeightBucketListFlush(parent: Bucket, children: BucketList, pivots: PivotTable)
+  requires WFPivots(pivots)
+  ensures WeightBucketList(BucketListFlush(parent, children, pivots))
+      <= WeightBucket(parent) + WeightBucketList(children)
+
+  lemma WeightBucketListClearEntry(blist: BucketList, i: int)
+  requires 0 <= i < |blist|
+  ensures WeightBucketList(blist[i := map[]]) <= WeightBucketList(blist)
+
+  lemma WeightSplitBucketInList(blist: BucketList, slot: int, pivot: Key)
+  requires 0 <= slot < |blist|
+  ensures WeightBucketList(SplitBucketInList(blist, slot, pivot))
+      == WeightBucketList(blist)
+
+  lemma WeightBucketListSlice(blist: BucketList, a: int, b: int)
+  requires 0 <= a <= b <= |blist|
+  ensures WeightBucketList(blist[a..b]) <= WeightBucketList(blist)
+
+  lemma WeightBucketListSuffix(blist: BucketList, a: int)
+  requires 0 <= a <= |blist|
+  ensures WeightBucketList(blist[a..]) <= WeightBucketList(blist)
+
+  lemma WeightBucketListConcat(left: BucketList, right: BucketList)
+  ensures WeightBucketList(left + right)
+      == WeightBucketList(left) + WeightBucketList(right)
+
+  lemma WeightMergeBucketsInList(blist: BucketList, slot: int, pivots: PivotTable)
+  requires 0 <= slot < |blist| - 1
+  requires WFBucketList(blist, pivots)
+  ensures WeightBucketList(MergeBucketsInList(blist, slot)) == WeightBucketList(blist)
+
+  lemma WeightJoinBucketList(blist: BucketList)
+  ensures WeightBucket(JoinBucketList(blist)) <= WeightBucketList(blist)
+
+  lemma WeightSplitBucketOnPivots(bucket: Bucket, pivots: seq<Key>)
+  ensures WeightBucketList(SplitBucketOnPivots(bucket, pivots)) == WeightBucket(bucket)
+}
