disk-betree/KMTable.i.dfy
@@ -1196,29 +1196,6 @@ module KMTable {
   //// Weight stuff
   /////////////////////////
 
-  function WeightKey(key: Key) : int
-  {
-    8 + |key|
-  }
-
-  function WeightKeySeq(keys: seq<Key>) : int
-  {
-    if |keys| == 0 then 0 else WeightKeySeq(DropLast(keys)) + WeightKey(Last(msgs))
-  }
-
-  function WeightMessage(msg: Message) : int
-  {
-    match msg {
-      Define(value) => |value|
-      Update(delta) => 0
-    }
-  }
-
-  function WeightMessageSeq(msgs: seq<Message>) : int
-  {
-    if |msgs| == 0 then 0 else WeightMessageSeq(DropLast(msgs)) + WeightMessage(Last(msgs))
-  }
-
   function Weight(kmt: KMTable) : int
   {
     WeightKeySeq(kmt.keys) + WeightMessageSeq(kmt.values)
